\textbf{Problem 7:}

\singlespacing

Let $P$ be the uniform distribution on the quarter disc

\singlespacing

\begin{equation}
    D = \{(x, y): x^2 + y^2 < 1,\quad x > 0,\quad y > 0\}
\end{equation}

\singlespacing

\textbf{part 1)}
\singlespacing

Let's find the marginal probability density function $p_1(x)$ that
is defined as:

\singlespacing

\begin{equation}
    p_1(x) = \int_{-\infty}^{\infty} p(x, y) \, dy
\end{equation}

\singlespacing

Where $p(x, y)$ is the joint probability density function of $P$.

\singlespacing

Let's find the joint probability density function $p(x, y)$:

\singlespacing

The uniform distribution on a quarter disc means that the probability density function (pdf) is constant over \( D \) and zero elsewhere. To find this constant, we need to ensure that the total probability over \( D \) is 1. The area of \( D \) is \( \frac{1}{4}\pi \), so the pdf \( p(x, y) \) is:

\[ p(x, y) = \frac{4}{\pi} \quad \text{for } (x, y) \in D \]

\singlespacing

Now we can find the marginal probability density function $p_1(x)$:

\singlespacing

Since \( p(x, y) \) is zero outside of \( D \), we only need to integrate over the values of \( y \) that correspond to a given \( x \) in \( D \). For a given \( x \) in \( D \), \( y \) ranges from 0 to \( \sqrt{1 - x^2} \). So the integral becomes:

\singlespacing

\begin{equation}
    p_1(x) = \int_{0}^{\sqrt{1 - x^2}} p(x, y) \, dy = \int_{0}^{\sqrt{1 - x^2}} \frac{4}{\pi} \, dy = \Big( \frac{4y}{\pi} \Big)\Big|_{0}^{\sqrt{1 - x^2}} = \frac{4\sqrt{1 - x^2}}{\pi} - \frac{4\cdot0}{\pi} = \frac{4\sqrt{1 - x^2}}{\pi}
\end{equation}

\singlespacing

Now generalizing for $x \in \mathbb{R}$, because the density function is zero outside of $[0, 1]$:

\singlespacing

\begin{equation}
    p_1(x) = \begin{cases}
        \frac{4\sqrt{1 - x^2}}{\pi} & \text{if } x \in [0, 1] \\
        0                           & \text{otherwise}
    \end{cases}
\end{equation}


\singlespacing
\textbf{part 2)}
\singlespacing

Now we can find the distribution function $F_1$, for that we need to integrate the density function $p_1$,
from $0$ to $x$, because the density function is zero outside of $[0, 1]$:

\singlespacing

We have three cases:

\singlespacing

\textbf{Case 1:} $x < 0$

\singlespacing

In this case $F_1(x) = 0$, because the density function is zero for $x < 0$:
\singlespacing

\textbf{Case 2:} $0 \leq x \leq 1$

\singlespacing

In this case $p_1(x) = \frac{4\sqrt{1 - x^2}}{\pi}$, so:

\singlespacing

\begin{equation}
    F_1(x) = \int_{0}^{x} \frac{4\sqrt{1 - u^2}}{\pi} \, du
\end{equation}

\singlespacing
Let's find the antiderivative of $F_1(x)$, and then we will evaluate it at $x$ and $0$:
\singlespacing
\begin{equation}
    \int \frac{4 \sqrt{1 - u^2}}{\pi} \, du
\end{equation}

\singlespacing
Factor out constants:
\singlespacing
\begin{equation}
    = \frac{4}{\pi} \int \sqrt{1 - u^2} \, du
\end{equation}

\singlespacing
For the integrand \(\sqrt{1 - u^2}\), substitute \(u = \sin(s)\) and \(du = \cos(s) \, ds\). Then \(\sqrt{1 - u^2} = \sqrt{1 - \sin^2(s)} = \cos(s)\) and \(s = \sin^{-1}(u)\):
\singlespacing
\begin{equation}
    = \frac{4}{\pi} \int \cos^2(s) \, ds
\end{equation}

\singlespacing
Write \(\cos^2(s)\) as \(\frac{1}{2} \cos(2 s) + \frac{1}{2}\):
\singlespacing
\begin{equation}
    = \frac{4}{\pi} \int \left( \frac{1}{2} \cos(2 s) + \frac{1}{2} \right) \, ds
\end{equation}

\singlespacing
Integrate the sum term by term and factor out constants:
\singlespacing
\begin{equation}
    = \frac{2}{\pi} \int \cos(2 s) \, ds + \frac{2}{\pi} \int 1 \, ds
\end{equation}

\singlespacing
For the integrand \(\cos(2 s)\), substitute \(p = 2 s\) and \(dp = 2 \, ds\):
\singlespacing
\begin{equation}
    = \frac{1}{\pi} \int \cos(p) \, dp + \frac{2}{\pi} \int 1 \, ds
\end{equation}

\singlespacing
The integral of \(\cos(p)\) is \(\sin(p)\):
\singlespacing
\begin{equation}
    = \frac{\sin(p)}{\pi} + \frac{2}{\pi} \int 1 \, ds
\end{equation}

\singlespacing
The integral of 1 is \(s\):
\singlespacing
\begin{equation}
    = \frac{\sin(p)}{\pi} + \frac{2 s}{\pi} + C
\end{equation}

\singlespacing
Substitute back for \(p = 2 s\):
\singlespacing
\begin{equation}
    = \frac{2 s + \sin(2 s)}{\pi} + C
\end{equation}

\singlespacing
Apply the double angle formula \(\sin(2 s) = 2 \sin(s) \cos(s)\):
\singlespacing
\begin{equation}
    = \frac{2 s + 2 \sin(s) \cos(s)}{\pi} + C
\end{equation}

\singlespacing
Express \(\cos(s)\) in terms of \(\sin(s)\) using \(\cos^2(s) = 1 - \sin^2(s)\):
\singlespacing
\begin{equation}
    = \frac{2 s + 2 \sin(s) \sqrt{1 - \sin^2(s)}}{\pi} + C
\end{equation}

\singlespacing
Substitute back for \(s = \sin^{-1}(u)\):
\singlespacing
\begin{equation}
    \text{Answer:} \quad = \frac{2 (\sqrt{1 - u^2} u + \sin^{-1}(u))}{\pi} + C
\end{equation}

\singlespacing

Now we can evaluate the antiderivative at $x$ and $0$:

\singlespacing

\begin{equation}
    F_1(x) = \Big( \frac{2 (\sqrt{1 - u^2} u + \sin^{-1}(u))}{\pi} \Big)\Big|_{0}^{x} = \frac{2 (\sqrt{1 - x^2} x + \sin^{-1}(x))}{\pi} - \frac{2 (\sqrt{1 - 0^2} 0 + \sin^{-1}(0))}{\pi} = \frac{2 (\sqrt{1 - x^2} x + \sin^{-1}(x))}{\pi}
\end{equation}

\singlespacing

\textbf{Case 3:} $x > 1$

\singlespacing

In this case $F_1(x) = 1$, because $x$ is greater than all the values where the density function is non-zero,
so the integral is equal to $1$.

\singlespacing

So, the distribution function $F_1$ of $P$ is:

\singlespacing

\begin{equation}
    F_1(x) = \begin{cases}
        0                                               & \text{if } x < 0           \\
        \frac{2 (\sqrt{1 - x^2} x + \sin^{-1}(x))}{\pi} & \text{if } 0 \leq x \leq 1 \\
        1                                               & \text{if } x > 1
    \end{cases}
\end{equation}

\singlespacing

\textbf{part 3)}
\singlespacing

Now let's evaluate $p_1$ at $x = \sqrt{1 - (\pi/4)^2}$:

\singlespacing

\begin{equation}
    p_1(\sqrt{1 - (\pi/4)^2}) = \frac{4\sqrt{1 - (\sqrt{1 - (\pi/4)^2})^2}}{\pi} = \frac{4\sqrt{1 - 1 + (\pi/4)^2}}{\pi} = \frac{4\sqrt{(\pi/4)^2}}{\pi} = \frac{4\pi/4}{\pi} = 1
\end{equation}