\textbf{Problem 3:}

\singlespacing

$P\left(\bigcup_{k=1}^{n} B_k\right) \leq \sum_{k=1}^{n} P(B_k),\quad B_1, B_2, \dots, B_n \in \mathcal{F}$

\singlespacing

We have the property that $P(A \cup B) = P(A) + P(B) - P(A \cap B)$, then:

\singlespacing

Let's prove it by induction:

\singlespacing

\textbf{Base case:} $n = 1$

\singlespacing

$P(B_1) \leq P(B_1)$

\singlespacing

\textbf{Inductive step:}

\singlespacing

We assume that the property holds for $n$ events, that is:

\singlespacing

$P\left(\bigcup_{k=1}^{n} B_k\right) \leq \sum_{k=1}^{n} P(B_k)$

\singlespacing

Now we need to prove that the property holds for $n + 1$ events, that is:

\singlespacing

$P\left(\bigcup_{k=1}^{n+1} B_k\right) \leq \sum_{k=1}^{n+1} P(B_k)$

\singlespacing

$P\left(\bigcup_{k=1}^{n} B_k \cup B_{n+1}\right) \leq \sum_{k=1}^{n} P(B_k) + P(B_{n+1})$

\singlespacing

$P\left(\bigcup_{k=1}^{n} B_k\right) + P(B_{n+1}) - P\left(\bigcup_{k=1}^{n} B_k \cap B_{n+1}\right) \leq \sum_{k=1}^{n} P(B_k) + P(B_{n+1})$

\singlespacing

$P\left(\bigcup_{k=1}^{n} B_k\right) - P\left(\bigcup_{k=1}^{n} B_k \cap B_{n+1}\right) \leq \sum_{k=1}^{n} P(B_k)$

\singlespacing

Because $P(A) \geq 0$ for any $A \in \mathcal{F}$, then $P\left(\bigcup_{k=1}^{n} B_k \cap B_{n+1}\right)$
is also positive, then we can remove it from the left side of the inequality, because
it will make the left side smaller, and the inequality will still hold:

\singlespacing

$P\left(\bigcup_{k=1}^{n} B_k\right) \leq \sum_{k=1}^{n} P(B_k)$

\singlespacing

Which is true by the inductive hypothesis.

\singlespacing

Then the property holds for $n + 1$ events, and by the principle of mathematical induction
the property holds for any $n \in \mathbb{N}$.