\textbf{Problem 2:}

\singlespacing

\begin{math}
    A=\begin{pmatrix}
        \begin{array}{cccccc}
            0 & 1 & 0 & 0 & 1 & 0 \\
            0 & 0 & 0 & 1 & 1 & 0 \\
            0 & 1 & 0 & 0 & 0 & 1
        \end{array}
    \end{pmatrix}\quad
    b=\begin{pmatrix}
        \begin{array}{cccccc}
            2  \\
            -1 \\
            1
        \end{array}
    \end{pmatrix}
\end{math}

\singlespacing

Solving the system:

\singlespacing

\begin{math}
    \begin{pmatrix}
        \begin{array}{cccccc|c}
            0 & 1 & 0 & 0 & 1 & 0 & 2  \\
            0 & 0 & 0 & 1 & 1 & 0 & -1 \\
            0 & 1 & 0 & 0 & 0 & 1 & 1
        \end{array}
    \end{pmatrix}\quad
\end{math}

\singlespacing

\begin{math}
    \begin{pmatrix}
        \begin{array}{cccccc|c}
            0 & 1 & 0 & 0 & 1  & 0 & 2  \\
            0 & 0 & 0 & 1 & 1  & 0 & -1 \\
            0 & 0 & 0 & 0 & -1 & 1 & -1
        \end{array}
    \end{pmatrix}\quad
    r3 = r3  + (-r1)
\end{math}

\singlespacing

We take free variables $x_1 = a$, $x_3 = b$, and $x_6 = c$ and
solve for the dependent variables $x_2$, $x_4$, and $x_5$:

\singlespacing

Extra equations:

\singlespacing

$x_2 + x_5 = 2$

$x_4 + x_5 = -1$

-$x_5 + x_6 = -1$

\singlespacing

Substituting $x_6 = c$:

\singlespacing

$x_2 + x_5 = 2$

$x_4 + x_5 = -1$

-$x_5 + c = -1$

\singlespacing

Solving:

\singlespacing

-$x_5 + c = -1$

$x_5 = c + 1$

\singlespacing

$x_2 + c + 1 = 2$

$x_2 = 1 - c$

\singlespacing

$x_4 + c + 1 = -1$

$x_4 = -2 - c$

\singlespacing

So the solution is:

\singlespacing

\begin{math}
    S = \left\{
    \begin{pmatrix}
        \begin{array}{c}
            a      \\
            1 - c  \\
            b      \\
            -2 - c \\
            c + 1  \\
            c
        \end{array}
    \end{pmatrix},\quad
    \forall a, b, c \in \mathbb{R}
    \right\}
\end{math}
