\textbf{Problem 6:}

\singlespacing

$\textbf{a)}$

\singlespacing

$\int \frac{e^{\sqrt{x}}}{\sqrt{x}}dx$

\singlespacing

We multiply the integral by $\frac{2}{2}$

\singlespacing

$\frac{2}{2}\int \frac{e^{\sqrt{x}}}{\sqrt{x}}dx$

\singlespacing

Because the linearity of the integral we can insert the constant inside the integral

\singlespacing

$2\cdot\int \frac{e^{\sqrt{x}}}{2\sqrt{x}}dx$

\singlespacing

Let's make some transformation

\singlespacing

$2\cdot\int e^{\sqrt{x}}\cdot \frac{1}{2\sqrt{x}}dx$

\singlespacing

Now let's apply the property $\int e^u \cdot u'dx  = e^u + C$

\singlespacing

And because $(x^n)' = nx^{n-1}$, then $\sqrt{x}' = (x^\frac{1}{2})' =
    \frac{1}{2}x^{(\frac{1}{2}-1)}  = \frac{1}{2}x^{(-\frac{1}{2})}= \frac{1}{2\cdot x^\frac{1}{2}}
    = \frac{1}{2\cdot \sqrt{x}}$

\singlespacing

Then $u = \sqrt{x}$ and $u' = \frac{1}{2\cdot \sqrt{x}}$, so:

\singlespacing

$2\cdot\int e^{\sqrt{x}}\cdot \frac{1}{2\sqrt{x}}dx = 2\cdot e^{\sqrt{x}} + C$

\singlespacing

Then the solution is $2\cdot e^{\sqrt{x}} + C$

\singlespacing
\singlespacing
\singlespacing

$\textbf{b)}$

\singlespacing

$\int x\sin{(x) }dx$

\singlespacing

Let's integrate by parts using the formula $\int u\cdot v'dx = u\cdot v - \int u'\cdot vdx$

\singlespacing

Let's take $u = x$ and $v' = \sin{(x)}$, so $u' = 1$ and $v = -\cos{(x)}$

\singlespacing

$\int x\sin{(x) }dx = x\cdot (-\cos{(x)}) - \int 1\cdot (-\cos{(x)})dx$

\singlespacing

$\int x\sin{(x) }dx = x\cdot (-\cos{(x)}) - \int (-\cos{(x)})dx$

\singlespacing

Extracting the constant $-1$ from the integral using the linearity property of the integral

\singlespacing

$\int x\sin{(x) }dx = -x\cdot \cos{(x)} + \int \cos{(x)}dx$

\singlespacing

Applying the property $\int \cos{(x)}dx = \sin{(x)} + C$

\singlespacing

$\int x\sin{(x) }dx = -x\cdot \cos{(x)} + \sin{(x)} + C$

\singlespacing

Then the solution is $-x\cdot \cos{(x)} + \sin{(x)} + C$